sketch out grow_file and grow_file_ok

src/SlowByteFile.v
@@ -230,8 +230,6 @@ Module SLOWBYTEFILE.
     exact tt.
   Qed.
 
-Check BFileRec.bf_getlen.
-
   Definition grow_blocks T fsxp inum nblock mscs rx : prog T := 
     let^ (mscs) <- For i < nblock
       Ghost [ mbase F Fm A f bytes ]
@@ -357,35 +355,74 @@ Check BFileRec.bf_getlen.
     apply LOG.activetxn_would_recover_old.
    Admitted.
 
-   Definition grow_file T fsxp inum off len mscs rx : prog T :=
-    let newsize := off + len in
-    let^ (mscs, oldattr) <- BFILE.bfgetattr fsxp.(FSXPLog) fsxp.(FSXPInode) inum mscs;
-    If (wlt_dec oldattr.(INODE.ISize) ($ newsize)) {
-      let curblocks := (cursize ^+ ($ valubytes) ^- $1) ^/ ($ valubytes)  in
-      let newblocks := (newsize ^+ ($ valubytes) ^- $1) ^/ ($ valubytes) in
-      let nblock := newblocks ^- curblocks in
-      let^ (mscs, ok) <- grow_blocks fsxp inum oldattr.(INODE.ISize) ($ nblock) mscs;
-      If (bool_dec ok true) {
-           mscs <- BFILE.bfsetattr fsxp.(FSXPLog) fsxp.(FSXPInode) inum
-                              (INODE.Build_iattr ($ newsize)
+   Hint Extern 1 ({{_}} progseq (grow_blocks _ _ _ _) _) => apply grow_blocks_ok : prog.
+
+   Definition grow_file T fsxp inum newlen mscs rx : prog T :=
+     let^ (mscs, oldattr) <- BFILE.bfgetattr fsxp.(FSXPLog) fsxp.(FSXPInode) inum mscs;
+     let curlen := oldattr.(INODE.ISize) in
+     let curblocks := (#curlen + valubytes - 1) / valubytes  in
+     let newblocks := (newlen + valubytes - 1) / valubytes in
+     let nblock := newblocks - curblocks in
+     let^ (mscs, ok) <- grow_blocks fsxp inum ($ nblock) mscs;
+     If (bool_dec ok true) {
+       mscs <- BFILE.bfsetattr fsxp.(FSXPLog) fsxp.(FSXPInode) inum
+                              (INODE.Build_iattr ($ newlen)
                                                  (INODE.IMTime oldattr)
                                                  (INODE.IType oldattr)) mscs;
-          rx ^(mscs, true)
-      } else {
-          rx ^(mscs, false)
-      }
-    } else {
-      rx ^(mscs, true)
-    }.
+       rx ^(mscs, true)
+     } else {
+       rx ^(mscs, false)
+     }.
+
+   Theorem grow_file_ok: forall fsxp inum newlen mscs,
+    {< m mbase F Fm A flist f bytes curlen,
+      PRE LOG.rep (FSXPLog fsxp) F (ActiveTxn mbase m) mscs *
+           [[ (Fm * BFILE.rep (FSXPBlockAlloc fsxp) (FSXPInode fsxp) flist)%pred (list2mem m) ]] *
+           [[ (A * #inum |-> f)%pred (list2nmem flist) ]] *
+           [[ bytes_rep f bytes  ]] *
+           [[ curlen = length bytes ]] *
+           [[ curlen < newlen ]]
+      POST RET:^(mscs, ok)
+           exists m', LOG.rep (FSXPLog fsxp) F (ActiveTxn mbase m') mscs *
+           ([[ ok = false ]] \/
+           [[ ok = true ]] * exists flist' f' bytes',
+           [[ (Fm * BFILE.rep (FSXPBlockAlloc fsxp) (FSXPInode fsxp) flist')%pred (list2mem m') ]] *
+           [[ (A * #inum |-> f')%pred (list2nmem flist') ]] *
+           [[ bytes' = (bytes ++ (repeat $0 (newlen-curlen))) ]] *
+           [[ rep bytes' f' ]])
+       CRASH LOG.would_recover_old (FSXPLog fsxp) F mbase 
+     >} grow_file fsxp inum newlen mscs.
+   Proof.
+     unfold grow_file, rep, bytes_rep.
+     step.
+     step.
+     instantiate (bytes0 := bytes).
+     admit. (* ?? maybe unification problem *)
+     step.
+     step.
+     step.
+     step.
+     step.
+     eapply pimpl_or_r; right; cancel.
+     admit. (* bytes' = (bytes ++ (repeat $0 (newlen-curlen))) etc.*)
+     step.
+   Admitted.
 
   Definition write_bytes T fsxp inum (off : nat) (data : list byte) mscs rx : prog T :=
-    let^ (mscs, ok) <- grow_file fsxp inum off (length data) mscs;
-    If (bool_dec ok true) {
-         mscs <- update_bytes fsxp inum off data mscs;
-         rx ^(mscs, ok)
+    let newlen := off + length data in
+    let^ (mscs, oldattr) <- BFILE.bfgetattr fsxp.(FSXPLog) fsxp.(FSXPInode) inum mscs;
+    let curlen := oldattr.(INODE.ISize) in      
+    If (wlt_dec curlen newlen) {
+         let^ (mscs, ok) <- grow_file fsxp inum newlen mscs;
+         If (bool_dec ok true) {
+           mscs <- update_bytes fsxp inum off data mscs;
+           rx ^(mscs, ok)
+        } else {
+          rx ^(mscs, false)
     } else {
-         rx ^(mscs, false)
-    }.
+        mscs <- update_bytes fsxp inum off data mscs;
+        rx ^(mscs, ok)
+    }
        
   Theorem write_bytes_ok: forall fsxp inum off len data mscs,
     {< m mbase F Fm A flist f bytes data0 Fx,
